Start filling in some possibly useful definitions

ironfleet/src/Dafny/Distributed/Services/Lock/AtomicTrace.i.dfy
@@ -182,6 +182,39 @@ module AtomicTrace_i {
         }
     }
 
+    predicate IsMover(q:QS_State)
+    {
+        var step  := q.environment.nextStep;
+            step.LEnvStepHostIos? 
+         && step.actor in q.servers    // It's one of our hosts
+         && (   |step.ios| == 0  // Host compute step
+             || (|step.ios| == 1 && (step.ios[0].LIoOpReceive? || step.ios[0].LIoOpSend?)))   // Normal send/receive
+    }
+
+    predicate IsNonMover(q:QS_State)
+    {
+        !IsMover(q)
+    }
+
+    function CanonicalAction(ios:IoTrace) : int
+        requires |ios| > 0;
+        requires LIoOpSeqCompatibleWithReduction(ios);
+        ensures  0 <= CanonicalAction(ios) < |ios|;
+    {
+        if exists i :: 0 <= i < |ios| && (ios[i].LIoOpTimeoutReceive? || ios[i].LIoOpReadClock?) then
+            // Choose the sole non-mover, if it exists
+            var i :| 0 <= i < |ios| && (ios[i].LIoOpTimeoutReceive? || ios[i].LIoOpReadClock?);
+            i
+        else if exists i :: 0 <= i < |ios| && ios[i].LIoOpSend? && (i == 0 || ios[i-1].LIoOpReceive?) then
+            // Else choose the left-most Send, if there are any sends
+            var i :| 0 <= i < |ios| && ios[i].LIoOpSend? && (i == 0 || ios[i-1].LIoOpReceive?);
+            i
+        else 
+            // Else choose the right-most receive (at this point, there are only receives left)
+            |ios| - 1
+    }
+            
+
 
 // TODO: Maybe we don't need ConcreteConfiguration
     ghost method MakeAtomicTrace(config:ConcreteConfiguration, qb:seq<QS_State>, external_io:SpecIoFilter) returns (qb':seq<QS_State>, db':seq<DS_State>) //, cm:seq<int>)
